coq/LC/Debruijn/F.v
@@ -2,7 +2,8 @@ Require Import
   Coq.Relations.Relations Coq.Relations.Relation_Operators
   Ssreflect.ssreflect Ssreflect.ssrfun Ssreflect.ssrbool Ssreflect.eqtype
   Ssreflect.ssrnat Ssreflect.seq
-  LCAC.lib.Relations_ext LCAC.lib.ssrnat_ext LCAC.lib.seq_ext.
+  LCAC.lib.Relations_ext LCAC.lib.seq_ext_base LCAC.lib.ssrnat_ext
+  LCAC.lib.seq_ext.
 
 Set Implicit Arguments.
 Unset Strict Implicit.
